.

GIT.v
@@ -1,12 +1,14 @@
-(* My formalization of ``Goedel's Incompleteness Theorems'' written by Raymond M. Smullyan *)
 From Coq.Bool Require Export Bool.
 From Coq.micromega Require Export Lia.
 From Coq.Lists Require Export List.
 From Coq.Arith Require Export PeanoNat.
 
-Section Chapter2.
+Module Smullyan's_Goedel's_Incompleteness_Theorems.
 
 Import ListNotations.
+
+Section Preliminaries.
+
 Lemma forallb_true_iff {A : Type} (f : A -> bool) :
   forall xs : list A,
   forallb f xs = true <-> (forall x : A, In x xs -> f x = true).
@@ -30,9 +32,11 @@ Proof.
         intros x H0; apply H; right; apply H0.
       }
 Qed.
+
 Definition fold_right_max_0 : list nat -> nat :=
   fold_right max 0
 .
+
 Lemma fold_right_max_0_in :
   forall ns : list nat,
   forall n : nat,
@@ -49,6 +53,7 @@ Proof.
       }
       lia.
 Qed.
+
 Lemma fold_right_max_0_app :
   forall ns1 : list nat,
   forall ns2 : list nat,
@@ -58,18 +63,25 @@ Proof.
   - simpl; intros n; lia.
   - simpl; intros n; rewrite IHns1; lia.
 Qed.
+
 Definition ensemble (A : Type) : Type :=
   A -> Prop
 .
+
 Definition member {A : Type} (x : A) (xs : ensemble A) : Prop :=
   xs x
 .
+
+Inductive empty {A : Type} : ensemble A :=
+.
+
 Inductive singletone {A : Type} : A -> ensemble A :=
 | In_singletone :
   forall x : A,
   forall xs : ensemble A,
   member x (singletone x)
 .
+
 Inductive union {A : Type} : ensemble A -> ensemble A -> ensemble A :=
 | In_union_left :
   forall x : A,
@@ -84,19 +96,157 @@ Inductive union {A : Type} : ensemble A -> ensemble A -> ensemble A :=
   member x xs2 ->
   member x (union xs1 xs2)
 .
+
 Definition insert {A : Type} (x1 : A) (xs2 : ensemble A) : ensemble A :=
   union xs2 (singletone x1)
 .
-Definition difference {A : Type} (xs1 : ensemble A) (xs2 : ensemble A) : ensemble A :=
-  fun x : A => member x xs1 /\ ~ member x xs2
+
+Definition intersection {A : Type} (xs1 : ensemble A) (xs2 : ensemble A) : ensemble A :=
+  fun x : A => member x xs1 /\ member x xs2
 .
+
+Definition completement {A : Type} (xs1 : ensemble A) : ensemble A :=
+  fun x : A => ~ member x  xs1
+.
+
+Definition difference {A : Type} (xs1 : ensemble A) (xs2 : ensemble A) : ensemble A :=
+  intersection xs1 (completement xs2)
+.
+
 Definition delete {A : Type} (x1 : A) (xs2 : ensemble A) : ensemble A :=
   difference xs2 (singletone x1)
 .
 
+Definition isSubsetOf {A : Type} (xs1 : ensemble A) (xs2 : ensemble A) : Prop :=
+  forall x : A, member x xs1 -> member x xs2
+.
+
+Lemma isSubsetOf_refl {A : Type} :
+  forall xs1 : ensemble A,
+  isSubsetOf xs1 xs1.
+Proof.
+  unfold isSubsetOf; intros xs1 x H; apply H.
+Qed.
+
+Lemma isSubsetOf_trans {A : Type} :
+  forall xs1 : ensemble A,
+  forall xs2 : ensemble A,
+  forall xs3 : ensemble A,
+  isSubsetOf xs1 xs2 ->
+  isSubsetOf xs2 xs3 ->
+  isSubsetOf xs1 xs3.
+Proof.
+  unfold isSubsetOf; intros xs1 xs2 xs3 H1 H2; apply (fun x : A => fun H0 : member x xs1 => H2 x (H1 x H0)).
+Qed.
+
+End Preliminaries.
+
+Section Chapter1.
+
+Class GoedelianLanguage (mathcalE : Type) : Type :=
+  { enum_mathcalE : nat -> mathcalE
+  ; mathcalE_is_enumerable : forall E : mathcalE, {n : nat | enum_mathcalE n = E}
+  ; isSentence : ensemble mathcalE
+  ; isProvable : ensemble mathcalE
+  ; isRefutable : ensemble mathcalE
+  ; isPredicate : ensemble mathcalE
+  ; apply_nat : mathcalE -> nat -> mathcalE
+  ; isTrue : ensemble mathcalE
+  ; onlyProvableIsSentence : isSubsetOf isProvable isSentence
+  ; onlyRefutableIsSentence : isSubsetOf isRefutable isSentence
+  ; apply_natForPredicate : forall h : mathcalE, isPredicate h -> forall n : nat, isSentence (apply_nat h n)
+  ; onlyTrueIsSentence : isSubsetOf isTrue isSentence
+  }
+.
+
+Definition diagonalizer (mathcalE : Type) `{mathcalE_is_goedelian : GoedelianLanguage mathcalE} : nat -> nat :=
+  fun n : nat => proj1_sig (mathcalE_is_enumerable (apply_nat (enum_mathcalE n) n))
+.
+
+Lemma diagonalizer_diagonalizes (mathcalE : Type) `{mathcalE_is_goedelian : GoedelianLanguage mathcalE} :
+  forall n : nat,
+  forall E : mathcalE,
+  enum_mathcalE n = E ->
+  enum_mathcalE (diagonalizer mathcalE n) = apply_nat E n.
+Proof.
+  intros n E H; unfold diagonalizer; subst; destruct (mathcalE_is_enumerable (apply_nat (enum_mathcalE n) n)) as [d_n]; simpl; tauto.
+Qed.
+
+Definition expressPredicate (mathcalE : Type) `{mathcalE_is_goedelian : GoedelianLanguage mathcalE} : mathcalE -> ensemble nat -> Prop :=
+  fun H : mathcalE => fun A : ensemble nat => forall n : nat, isTrue (apply_nat H n) <-> member n A
+.
+
+Definition is_expressible (mathcalE : Type) `{mathcalE_is_goedelian : GoedelianLanguage mathcalE} : ensemble nat -> Prop :=
+  fun A : ensemble nat => exists H : mathcalE, expressPredicate mathcalE H A
+.
+
+Inductive StarOf (mathcalE : Type) `{mathcalE_is_goedelian : GoedelianLanguage mathcalE} : ensemble nat -> ensemble nat :=
+| InStarOf :
+  forall ns : ensemble nat,
+  forall n : nat,
+  member (diagonalizer mathcalE n) ns ->
+  member n (StarOf mathcalE ns)
+.
+
+Definition isCorrect (mathcalE : Type) `{mathcalE_is_goedelian : GoedelianLanguage mathcalE} : Prop :=
+  isSubsetOf isProvable isTrue /\ isSubsetOf (intersection isRefutable isTrue) empty
+.
+
+Inductive P (mathcalE : Type) `{mathcalE_is_goedelian : GoedelianLanguage mathcalE} : ensemble nat :=
+| InP :
+  forall n : nat,
+  isProvable (enum_mathcalE n) ->
+  member n (P mathcalE)
+.
+
+Theorem After_Goedel_with_shades_of_Tarski (mathcalE : Type) `{mathcalE_is_goedelian : GoedelianLanguage mathcalE} :
+  isCorrect mathcalE ->
+  is_expressible mathcalE (StarOf mathcalE (completement (P mathcalE))) ->
+  exists E : mathcalE, isTrue E /\ ~ isProvable E.
+Proof.
+  intros mathcalE_is_correct StarOf_complement_P_is_expressible.
+  destruct StarOf_complement_P_is_expressible as [H H_express_StarOf_complement_P].
+  destruct (mathcalE_is_enumerable H) as [n n_is_the_goedel_number_of_H].
+  assert (diagonalization_of_n_is_true_iff_n_is_in_StarOf_complement_of_P : isTrue (enum_mathcalE (diagonalizer mathcalE n)) <-> member n (StarOf mathcalE (completement (P mathcalE)))).
+  { unfold expressPredicate in H_express_StarOf_complement_P.
+    rewrite (diagonalizer_diagonalizes mathcalE n H n_is_the_goedel_number_of_H).
+    apply H_express_StarOf_complement_P.
+  }
+  assert (n_in_StarOf_complement_of_P_iff_diagonalization_of_n_is_not_Provable : member n (StarOf mathcalE (completement (P mathcalE))) <-> ~ isProvable (enum_mathcalE (diagonalizer mathcalE n))).
+  { constructor.
+    - intros n_in_StarOf_complement_of_P diagonalization_of_n_is_not_Provable.
+      inversion n_in_StarOf_complement_of_P as [A n' diagonalization_of_n_is_in_A A_is_complement_of_P n_is_n']; subst n'.
+      contradiction diagonalization_of_n_is_in_A.
+      apply InP.
+      apply diagonalization_of_n_is_not_Provable.
+    - intros diagonalization_of_n_is_not_Provable.
+      apply InStarOf.
+      intros diagonalization_of_n_is_in_P.
+      contradiction diagonalization_of_n_is_not_Provable.
+      inversion diagonalization_of_n_is_in_P as [n' diagonalization_of_n_is_Provable n_is_n']; subst n'.
+      apply diagonalization_of_n_is_Provable.
+  }
+  assert (diagonalization_of_n_is_not_Provable : ~ isProvable (enum_mathcalE (diagonalizer mathcalE n))).
+  { intros diagonalization_of_n_is_Provable.
+    destruct mathcalE_is_correct as [Provable_implies_true Refutable_implies_false].
+    assert (diagonalization_of_n_is_True : isTrue (enum_mathcalE (diagonalizer mathcalE n))).
+    { apply Provable_implies_true.
+      apply diagonalization_of_n_is_Provable.
+    }
+    tauto.
+  }
+  exists (enum_mathcalE (diagonalizer mathcalE n)).
+  tauto.
+Qed.
+
+End Chapter1.
+
+Section Chapter2.
+
 Definition vr : Set :=
   nat
 .
+
 Inductive tm : Set :=
 | ivar_tm : vr -> tm
 | zero_tm : tm
@@ -105,6 +255,7 @@ Inductive tm : Set :=
 | mult_tm : tm -> tm -> tm
 | expo_tm : tm -> tm -> tm
 .
+
 Inductive form : Set :=
 | eqn_form : tm -> tm -> form
 | leq_form : tm -> tm -> form
@@ -120,6 +271,7 @@ Lemma vr_eq_dec :
 Proof.
   apply Nat.eq_dec.
 Qed.
+
 Fixpoint occursFreeIn_tm (z : vr) (t : tm) : bool :=
   match t with
   | ivar_tm x => if vr_eq_dec z x then true else false
@@ -130,6 +282,7 @@ Fixpoint occursFreeIn_tm (z : vr) (t : tm) : bool :=
   | expo_tm t1 t2 => occursFreeIn_tm z t1 || occursFreeIn_tm z t2
   end
 .
+
 Fixpoint occursFreeIn_form (z : vr) (f : form) : bool :=
   match f with
   | eqn_form t1 t2 => occursFreeIn_tm z t1 || occursFreeIn_tm z t2
@@ -139,6 +292,7 @@ Fixpoint occursFreeIn_form (z : vr) (f : form) : bool :=
   | all_form x f1 => if vr_eq_dec z x then false else occursFreeIn_form z f1
   end
 .
+
 Fixpoint getFreeVars_tm (t : tm) : list vr :=
   match t with
   | ivar_tm x => [x]
@@ -149,6 +303,7 @@ Fixpoint getFreeVars_tm (t : tm) : list vr :=
   | expo_tm t1 t2 => getFreeVars_tm t1 ++ getFreeVars_tm t2
   end
 .
+
 Theorem the_rule_of_getFreeVars_tm :
   forall t : tm,
   forall x : vr,
@@ -177,6 +332,7 @@ Proof.
   - intros vr; simpl; rewrite orb_true_iff; rewrite in_app_iff; rewrite IHt1; rewrite IHt2; reflexivity.
   - intros vr; simpl; rewrite orb_true_iff; rewrite in_app_iff; rewrite IHt1; rewrite IHt2; reflexivity.
 Qed.
+
 Fixpoint getFreeVars_form (f : form) : list vr :=
   match f with
   | eqn_form t1 t2 => getFreeVars_tm t1 ++ getFreeVars_tm t2
@@ -186,6 +342,7 @@ Fixpoint getFreeVars_form (f : form) : list vr :=
   | all_form x f1 => remove vr_eq_dec x (getFreeVars_form f1)
   end
 .
+
 Theorem the_rule_of_getFreeVars_form :
   forall f : form,
   forall x : vr,
@@ -218,9 +375,11 @@ Qed.
 Definition value_of_N : Set :=
   nat
 .
+
 Definition value_assignment : Set :=
   vr -> value_of_N
 .
+
 Fixpoint eval_tm (va : value_assignment) (t : tm) : value_of_N :=
   match t with
   | ivar_tm x => va x
@@ -231,6 +390,7 @@ Fixpoint eval_tm (va : value_assignment) (t : tm) : value_of_N :=
   | expo_tm t1 t2 => (eval_tm va t1)^(eval_tm va t2)
   end
 .
+
 Lemma eval_tm_extensionality :
   forall t : tm,
   forall va1 : value_assignment,
@@ -267,6 +427,7 @@ Proof.
     intros x H0; apply H; apply orb_true_iff; tauto.
     intros x H0; apply H; apply orb_true_iff; tauto.
 Qed.
+
 Fixpoint eval_form (va : value_assignment) (f : form) : Prop :=
   match f with
   | eqn_form t1 t2 => eval_tm va t1 = eval_tm va t2
@@ -276,6 +437,7 @@ Fixpoint eval_form (va : value_assignment) (f : form) : Prop :=
   | all_form x f1 => forall val : value_of_N, eval_form (fun z : vr => if vr_eq_dec x z then val else va z) f1
   end
 .
+
 Lemma eval_form_extensionality :
   forall f : form,
   forall va1 : value_assignment,
@@ -327,12 +489,14 @@ Proof.
       - apply H0.
     }
 Qed.
+
 Fixpoint make_numeral (n : value_of_N) : tm :=
   match n with
   | 0 => zero_tm
   | S n' => succ_tm (make_numeral n')
   end
 .
+
 Lemma eval_tm_make_numeral :
   forall n : value_of_N,
   forall va : value_assignment,
@@ -346,12 +510,14 @@ Qed.
 Definition substitution : Set :=
   list (vr * tm)
 .
+
 Fixpoint substitute_vr (sigma : substitution) (x : vr) : tm :=
   match sigma with
   | [] => ivar_tm x
   | (x1, tm1) :: sigma' => if vr_eq_dec x x1 then tm1 else substitute_vr sigma' x
   end
 .
+
 Fixpoint substitute_tm (sigma : substitution) (t : tm) : tm :=
   match t with
   | ivar_tm x => substitute_vr sigma x
@@ -362,6 +528,7 @@ Fixpoint substitute_tm (sigma : substitution) (t : tm) : tm :=
   | expo_tm t1 t2 => expo_tm (substitute_tm sigma t1) (substitute_tm sigma t2)
   end
 .
+
 Theorem substitute_tm_preserves_eval_tm :
   forall t : tm,
   forall sigma : substitution,
@@ -376,9 +543,11 @@ Proof.
   - intros sigma va; simpl; rewrite IHt1; rewrite IHt2; reflexivity.
   - intros sigma va; simpl; rewrite IHt1; rewrite IHt2; reflexivity.
 Qed.
+
 Definition getMaxNumOfFreeVars_tm (t : tm) : vr :=
   fold_right_max_0 (getFreeVars_tm t)
 .
+
 Lemma getMaxNumOfFreeVars_tm_lt :
   forall t : tm,
   forall x : vr,
@@ -401,15 +570,19 @@ Proof.
     + apply IHt1; lia.
     + apply IHt2; lia.
 Qed.
+
 Definition isFreshVarIn_substitute_tm (sigma : substitution) (z : vr) (t : tm) : Prop :=
   forallb (fun x : vr => negb (occursFreeIn_tm z (substitute_vr sigma x))) (getFreeVars_tm t) = true
 .
+
 Definition isFreshVarIn_substitute_form (sigma : substitution) (z : vr) (f : form) : Prop :=
   forallb (fun x : vr => negb (occursFreeIn_tm z (substitute_vr sigma x))) (getFreeVars_form f) = true
 .
+
 Definition chi (sigma : substitution) (f : form) : vr :=
   S (fold_right_max_0 (map (fun x : vr => getMaxNumOfFreeVars_tm (substitute_vr sigma x)) (getFreeVars_form f)))
 .
+
 Theorem the_rule_of_chi :
   forall f : form,
   forall sigma : substitution,
@@ -439,6 +612,7 @@ Proof.
   unfold isFreshVarIn_substitute_form; intros f sigma; apply forallb_true_iff.
   intros x H; apply negb_true_iff; apply claim1; apply the_rule_of_getFreeVars_form; apply H.
 Qed.
+
 Fixpoint substitute_form (sigma : substitution) (f : form) : form :=
   match f with
   | eqn_form t1 t2 => eqn_form (substitute_tm sigma t1) (substitute_tm sigma t2)
@@ -450,6 +624,7 @@ Fixpoint substitute_form (sigma : substitution) (f : form) : form :=
     all_form z (substitute_form ((x, ivar_tm z) :: sigma) f1)
   end
 .
+
 Theorem substitute_form_preserves_eval_form :
   forall f : form,
   forall sigma : substitution,
@@ -499,6 +674,7 @@ Proof.
         + reflexivity.
     }
 Qed.
+
 Lemma substitute_tm_make_numeral :
   forall n : value_of_N,
   forall sigma : substitution,
@@ -510,7 +686,9 @@ Proof.
 Qed.
 
 Ltac simpl_eval_tm_make_numeral := repeat (rewrite substitute_tm_make_numeral); repeat (rewrite eval_tm_make_numeral).
+
 Ltac simpl_in_eval_tm_make_numeral H := repeat (rewrite substitute_tm_make_numeral in H); repeat (rewrite eval_tm_make_numeral in H).
+
 Lemma occursFreeIn_tm_make_numeral :
   forall val : value_of_N,
   forall x : vr,
@@ -520,7 +698,9 @@ Proof.
   - intros x; simpl; reflexivity.
   - intros x; simpl; rewrite (IHval x); reflexivity.
 Qed.
+
 Ltac simplify_make_numeral := repeat (rewrite substitute_tm_make_numeral); repeat (apply occursFreeIn_tm_make_numeral).
+
 Lemma vr_eq_dec_is_Nat_eq_dec {A : Type} :
   forall x1 : A,
   forall x2 : A,
@@ -537,15 +717,20 @@ Proof.
     + contradiction.
     + reflexivity.
 Qed.
+
 Ltac eval_vr_eq_dec := repeat (rewrite vr_eq_dec_is_Nat_eq_dec; simpl).
+
 Ltac eval_in_vr_eq_dec H := repeat (rewrite vr_eq_dec_is_Nat_eq_dec in H; simpl in H).
+
 Ltac auto_show_it_is_sentence := tryif (apply orb_false_iff; constructor) then auto_show_it_is_sentence else (eval_vr_eq_dec; simplify_make_numeral).
+
 Fixpoint relation_of_arity (n : nat) : Type :=
   match n with
   | 0 => Prop
   | S n' => value_of_N -> relation_of_arity n'
   end
 .
+
 Fixpoint lift_relation (n : nat) : relation_of_arity (S n) -> nat -> relation_of_arity n :=
   match n as n0 return relation_of_arity (S n0) -> nat -> relation_of_arity n0 with
   | 0 =>
@@ -559,6 +744,7 @@ Fixpoint lift_relation (n : nat) : relation_of_arity (S n) -> nat -> relation_of
     lift_relation n' (pred val') val 
   end
 .
+
 Fixpoint express_relation (n : nat) : form -> relation_of_arity n -> Prop :=
   match n as n0 return form -> relation_of_arity n0 -> Prop with
   | 0 =>
@@ -571,6 +757,7 @@ Fixpoint express_relation (n : nat) : form -> relation_of_arity n -> Prop :=
     forall val : value_of_N, express_relation n' (substitute_form [(n', make_numeral val)] f) (lift_relation n' pred val)
   end
 .
+
 Example express_relation_example1 :
   express_relation 2 (leq_form (ivar_tm 0) (ivar_tm 1)) (fun x0 : value_of_N => fun x1 : value_of_N => x0 <= x1).
 Proof.
@@ -583,12 +770,14 @@ Proof.
       assert (H0 := H (fun _ : vr => 0)).
       eval_in_vr_eq_dec H0; simpl_in_eval_tm_make_numeral H0; tauto.
 Qed.
+
 Fixpoint function_of_arity (n : nat) : Type :=
   match n with
   | 0 => value_of_N
   | S n' => value_of_N -> function_of_arity n'
   end
 .
+
 Fixpoint lift_function (n : nat) : function_of_arity (S n) -> nat -> function_of_arity n :=
   match n as n0 return function_of_arity (S n0) -> nat -> function_of_arity n0 with
   | 0 =>
@@ -602,6 +791,7 @@ Fixpoint lift_function (n : nat) : function_of_arity (S n) -> nat -> function_of
     lift_function n' (func val') val 
   end
 .
+
 Fixpoint express_function (n : nat) : form -> function_of_arity n -> Prop :=
   match n as n0 return form -> function_of_arity n0 -> Prop with
   | 0 =>
@@ -616,6 +806,7 @@ Fixpoint express_function (n : nat) : form -> function_of_arity n -> Prop :=
     forall val : value_of_N, express_function n' (substitute_form [(n, make_numeral val)] f) (lift_function n' func val)
   end
 .
+
 Example express_function_example1 :
   express_function 3 (eqn_form (ivar_tm 0) (plus_tm (ivar_tm 1) (plus_tm (ivar_tm 2) (ivar_tm 3)))) (fun x1 : value_of_N => fun x2 : value_of_N => fun x3 : value_of_N => x1 + (x2 + x3)).
 Proof.
@@ -630,3 +821,5 @@ Proof.
 Qed.
 
 End Chapter2.
+
+End Smullyan's_Goedel's_Incompleteness_Theorems.
